Guest.lean
@@ -12,6 +12,7 @@ import Guest.StepCalculus
 import Guest.Termination
 import Guest.Memory
 import Guest.Expressions
+import Guest.Gas
 import Guest.FunctionTermination
 import Guest.StepBound
 import Guest.AstParse
